Changes for simplified model checking

CertifyingDatalog/Basic.lean
@@ -280,3 +280,14 @@ lemma List.foldl_union_subset_set {A B: Type} [DecidableEq B] (l: List A) (f: A 
     rw [ih]
     simp
     tauto
+
+
+-- added based on https://leanprover.zulipchat.com/#narrow/stream/113488-general/topic/finset.2Efilter
+noncomputable def Finset.filter_nc (p: A → Prop) (S: Finset A):= @Finset.filter A p (Classical.decPred p) S
+
+lemma Finset.mem_filter_nc (a:A) (p: A → Prop) (S: Finset A): a ∈ Finset.filter_nc p S ↔ p a ∧ a ∈ S :=
+by
+  unfold filter_nc
+  have dec: DecidablePred p := Classical.decPred p
+  simp [Finset.mem_filter]
+  rw [And.comm]
