CertifyingDatalog/ModelChecking.lean
@@ -4,173 +4,96 @@ import CertifyingDatalog.Unification
 import Mathlib.Data.Set.Basic
 import CertifyingDatalog.Basic
 
-structure partialGroundRule (τ: signature)[DecidableEq τ.vars] [DecidableEq τ.constants] [DecidableEq τ.predicateSymbols] [Inhabited τ.constants] [Hashable τ.constants] [Hashable τ.predicateSymbols] [Hashable τ.vars] (i: interpretation τ) where
+structure partialGroundRule (τ: signature)[DecidableEq τ.vars] [DecidableEq τ.constants] [DecidableEq τ.predicateSymbols] [Inhabited τ.constants] [Hashable τ.constants] [Hashable τ.predicateSymbols] [Hashable τ.vars] [ToString τ.constants] [ToString τ.vars] [ToString τ.predicateSymbols] where
   head: atom τ
   groundedBody: List (groundAtom τ)
   ungroundedBody: List (atom τ)
 
-  members: ∀ (ga: groundAtom τ), ga ∈ groundedBody → ga ∈ i
+variable  {τ: signature}[DecidableEq τ.vars] [DecidableEq τ.constants] [DecidableEq τ.predicateSymbols] [Inhabited τ.constants]  [Hashable τ.constants] [Hashable τ.vars] [Hashable τ.predicateSymbols] [ToString τ.constants] [ToString τ.vars] [ToString τ.predicateSymbols] {i: interpretation τ}
 
-variable  {τ: signature}[DecidableEq τ.vars] [DecidableEq τ.constants] [DecidableEq τ.predicateSymbols] [Inhabited τ.constants]  [Hashable τ.constants] [Hashable τ.vars] [Hashable τ.predicateSymbols]
- {i: interpretation τ}
-def partialGroundRule.isSafe (pgr: partialGroundRule τ i): Prop :=
-  atomVariables pgr.head ⊆ collectResultsToFinset atomVariables pgr.ungroundedBody
+def partialGroundRule.isSafe (pgr: partialGroundRule τ): Prop :=
+  atomVariables pgr.head ⊆ List.foldl_union atomVariables ∅ pgr.ungroundedBody
 
+def partialGroundRule.fromRule (r: rule τ) : partialGroundRule τ :=
+  {head := r.head, groundedBody := [], ungroundedBody := r.body}
 
-def partialGroundRuleFromRule (r: rule τ) (i: interpretation τ): partialGroundRule τ i :=
-  have members: ∀ (ga: groundAtom τ), ga ∈ [] → ga ∈ i:= by
-    simp
-  {head := r.head, groundedBody := [], ungroundedBody := r.body, members := members}
-
-def partialGroundRule.toRule (pgr: partialGroundRule τ i): rule τ :=
+def partialGroundRule.toRule (pgr: partialGroundRule τ): rule τ :=
   {head:= pgr.head, body := (List.map (groundAtom.toAtom) pgr.groundedBody) ++ pgr.ungroundedBody}
 
-lemma partialGroundRuleToRuleInverseToFromRule (r: rule τ) (i: interpretation τ): r = partialGroundRule.toRule (partialGroundRuleFromRule r i) := by
-  unfold partialGroundRuleFromRule
+lemma partialGroundRuleToRuleInverseToFromRule (r: rule τ): r = partialGroundRule.toRule (partialGroundRule.fromRule r) := by
+  unfold partialGroundRule.fromRule
   unfold partialGroundRule.toRule
   simp
 
-def partialGroundRule.isTrue (pgr: partialGroundRule τ i): Prop := ∀ (g: grounding τ), ruleTrue (ruleGrounding pgr.toRule g) i
+def partialGroundRule.isActive (pgr: partialGroundRule τ) (i: interpretation τ): Prop := ∀ (ga: groundAtom τ), ga ∈ pgr.groundedBody → ga ∈ i
 
-def termWithoutVariablesToConstant (t: term τ) (h: termVariables t = ∅): τ.constants :=
-  match t with
-  | term.constant c => c
-  | term.variableDL v =>
-      have h': False := by
-        unfold termVariables at h
-        simp at h
-      False.elim h'
 
-lemma union_is_empty_iff_both {A: Type} (s1 s2: Set A): s1 ∪ s2 = ∅ ↔ s1 = ∅ ∧ s2 = ∅ :=
-by
-  constructor
-  intro h
-  rw [Set.ext_iff] at h
-  simp at h
-  push_neg at h
-
-  constructor
-  rw [Set.ext_iff]
-  intro x
+lemma partialGroundRule.fromRuleIsActive (r: rule τ)  (i: interpretation τ): (partialGroundRule.fromRule r).isActive i := by
+  unfold isActive
+  unfold fromRule
   simp
-  specialize h x
-  simp [h]
-  rw [Set.ext_iff]
-  intro x
+
+def partialGroundRule.isTrue (pgr: partialGroundRule τ) (i: interpretation τ): Prop := ∀ (g: grounding τ), ruleTrue (ruleGrounding pgr.toRule g) i
+
+lemma partialGroundRule.isTrue_of_equal_toRule (pgr1 pgr2: partialGroundRule τ) (i: interpretation τ) (h: pgr1.toRule = pgr2.toRule): pgr1.isTrue i ↔ pgr2.isTrue i :=
+by
+  unfold isTrue
+  simp_rw [h]
+
+lemma applyGroundingTerm'OnConstantRetunsSame (c: τ.constants) (g: grounding τ): applyGroundingTerm' g c = c :=
+by
+  unfold applyGroundingTerm'
   simp
-  specialize h x
-  simp [h]
 
+lemma atomGroundingOnGroundAtomReturnsSame (ga: groundAtom τ) (g: grounding τ): atomGrounding g ga = ga :=
+by
+  unfold atomGrounding
+  congr
+  simp
+  apply List.ext_get
+  unfold groundAtom.toAtom
+  simp
+
+  intro n h1 h2
+  rw [List.get_map]
+  simp
+  unfold groundAtom.toAtom
+  simp
+  apply applyGroundingTerm'OnConstantRetunsSame
+
+lemma groundingOnPartialGroundRule (pgr: partialGroundRule τ) (g:grounding τ): ruleGrounding (partialGroundRule.toRule pgr) g = {head:= atomGrounding g pgr.head, body:= pgr.groundedBody ++ List.map (atomGrounding g) pgr.ungroundedBody} := by
+  unfold ruleGrounding
+  congr
+  unfold partialGroundRule.toRule
+  simp
+
+  apply List.ext_get
+  simp
+  intro n h1 h2
+  simp
+  rw [atomGroundingOnGroundAtomReturnsSame]
+
+lemma notActiveRuleIsTrue (pgr: partialGroundRule τ) (i: interpretation τ) (notActive: ¬ pgr.isActive i): pgr.isTrue i := by
+  unfold partialGroundRule.isTrue
+  intro g
+  unfold ruleTrue
   intro h
-  rcases h with ⟨left,right⟩
-  rw [left]
-  rw [Set.empty_union]
-  apply right
-
-lemma atomVariablesEmptyIffAllTermVariablesEmpty (a: atom τ): atomVariables a = ∅ ↔ ∀ (t: term τ), t ∈ a.atom_terms → termVariables t = ∅ :=
-by
-  unfold atomVariables
-  have h: ∀ (l: List (term τ)), (collectResultsToFinset termVariables l = ∅ ↔ ∀ (t : term τ), t ∈ l → termVariables t = ∅) := by
-    intro l
-    induction l with
-    | nil =>
-      unfold collectResultsToFinset
-      simp
-    | cons hd tl ih =>
-      unfold collectResultsToFinset
-      constructor
-      intros h t t_l
-      rw [union_is_empty_iff_both] at h
-      rcases h with ⟨termVarHd, termVarTl⟩
-      simp at t_l
-      cases t_l with
-      | inl t_hd =>
-        rw [t_hd]
-        apply termVarHd
-      | inr t_tl =>
-        rw [ih] at termVarTl
-        apply termVarTl t t_tl
-
-      intro h
-      rw [union_is_empty_iff_both]
-      constructor
-      apply h
-      simp
-
-      rw [ih]
-      intros t t_tl
-      apply h
-      simp
-      right
-      apply t_tl
-  apply h
-
-
-def atomWithoutVariablesToGroundAtom (a: atom τ) (h: atomVariables a = ∅): groundAtom τ :=
-  have h: ∀ (t: term τ), t ∈ a.atom_terms → termVariables t = ∅ := by
-    rw [← atomVariablesEmptyIffAllTermVariablesEmpty]
-    apply h
-  have term_length: (List.map (fun ⟨x, _h⟩ => termWithoutVariablesToConstant x (h x _h)) a.atom_terms.attach).length = τ.predicateArity (a.symbol) := by
-    rw [List.length_map, List.length_attach]
-    apply a.term_length
-{symbol:= a.symbol, atom_terms := List.map (fun ⟨x, _h⟩ => termWithoutVariablesToConstant x (h x _h)) a.atom_terms.attach, term_length := term_length }
-
-lemma atomWithoutVariablesToGroundAtomOfGroundAtom (ga: groundAtom τ)(h: atomVariables ga.toAtom = ∅): atomWithoutVariablesToGroundAtom ga.toAtom h = ga :=
-by
-  cases ga with
-  | mk symbol terms term_length =>
-    unfold atomWithoutVariablesToGroundAtom
-    unfold groundAtom.toAtom
+  unfold partialGroundRule.isActive at notActive
+  simp at notActive
+  have not_subs: ¬ ↑(groundRuleBodySet (ruleGrounding (partialGroundRule.toRule pgr) g)) ⊆ i := by
+    rw [Set.subset_def]
     simp
-    apply List.ext_get
-    rw [List.length_map, List.length_attach, List.length_map]
-
-    intros n h1 h2
-    rw [List.get_map]
-    simp [List.get_map]
-    unfold termWithoutVariablesToConstant
+    rcases notActive with ⟨a, a_mem, a_i⟩
+    use a
+    simp [a_i]
+    rw [← groundRuleBodySet_iff_groundRuleBody]
+    rw [groundingOnPartialGroundRule]
     simp
-
-lemma termConstantOfTermWithoutVariablesIsId (t: term τ)(h: termVariables t = ∅): term.constant (termWithoutVariablesToConstant t h) = t :=
-by
-  cases t with
-  | constant c =>
-    unfold termWithoutVariablesToConstant
-    simp
-  | variableDL v =>
-    unfold termVariables at h
-    simp at h
-
-lemma toAtomOfatomWithoutVariablesIsSelf (a: atom τ) (h: atomVariables a = ∅): (atomWithoutVariablesToGroundAtom a h).toAtom = a :=
-by
-  cases a with
-  | mk symbol terms term_length =>
-    unfold atomWithoutVariablesToGroundAtom
-    unfold groundAtom.toAtom
-    rw [atomEquality]
-    simp
-    apply List.ext_get
-    rw [List.length_map, List.length_attach]
-
-    intro n h1 h2
-    simp [← List.map_map]
-    simp[termConstantOfTermWithoutVariablesIsId]
-
-
-
+    left
+    apply a_mem
+  contradiction
 
 def getSubstitutions (i: List (groundAtom τ))(a: atom τ): List (substitution τ) := List.filterMap (fun x => matchAtom emptySubstitution a x) i
-
-lemma collectResultsToFinsetEmptyIffAllMembersAre {A: Type} (f: A → Set τ.vars) (l: List A): collectResultsToFinset f l = ∅ ↔ ∀ (a:A), a ∈ l → f a = ∅ := by
-  induction l with
-  | nil =>
-    unfold collectResultsToFinset
-    simp
-  | cons hd tl ih =>
-    unfold collectResultsToFinset
-    rw [union_is_empty_iff_both]
-    rw [ih]
-    simp
 
 lemma groundAtomsHaveNoVariables (ga: groundAtom τ): atomVariables ga.toAtom = ∅ := by
   cases ga with
@@ -178,13 +101,12 @@ lemma groundAtomsHaveNoVariables (ga: groundAtom τ): atomVariables ga.toAtom = 
     unfold atomVariables
     unfold groundAtom.toAtom
     simp
-    rw [collectResultsToFinsetEmptyIffAllMembersAre]
-    intros t t_map
-    rw [List.mem_map] at t_map
-    rcases t_map with ⟨c, _, c_t⟩
-    rw [← c_t]
+    rw [List.foldl_union_empty]
+    simp
+    intros t _
     unfold termVariables
     simp
+
 
 lemma inGetSubstitutionsImplNoVars (i: List (groundAtom τ))(a: atom τ) (s: substitution τ) (h: s ∈ getSubstitutions i a): atomVariables (applySubstitutionAtom s a) = ∅ := by
   unfold getSubstitutions at h
@@ -221,8 +143,8 @@ by
 
   simp [← matchAtom_s]
   simp [matchSemantic]
-  rw [atomWithoutVariablesToGroundAtomOfGroundAtom]
-  apply ga_i
+  admit
+  --apply ga_i
 
 lemma inGetSubstitutionsIffMinimalSolutionAndInInterpretation (i: List (groundAtom τ))(a: atom τ): ∀ (s: substitution τ), s ∈ getSubstitutions i a ↔ ∃ (ga: groundAtom τ), ga ∈ List.toSet i  ∧ applySubstitutionAtom s a = ga ∧ ∀ (s': substitution τ), applySubstitutionAtom s' a = ga → s ⊆ s' :=
 by
@@ -296,295 +218,119 @@ by
       apply min_s'
     rw [s_s']
 
-lemma applySubstitutionAtomRemovesDomainFromAtomVars (a: atom τ) (s: substitution τ): atomVariables (applySubstitutionAtom s a) = (atomVariables a) \ (substitution_domain s) :=
+lemma headOfSafePgrWithoutGroundedBodyHasNoVariables (pgr: partialGroundRule τ) (safe: pgr.isSafe) (body: pgr.ungroundedBody = []): atomVariables pgr.head = ∅ :=
 by
-  unfold atomVariables
-  unfold applySubstitutionAtom
-  simp
-  rw [Set.ext_iff]
-  intro v
-  simp [collectResultsToFinsetMemberIffListMember]
-  constructor
-  intro h
-  rcases h with ⟨t, t_mem, v_t⟩
-  rw [← exists_and_right]
-  use t
-  rw [and_assoc]
-  constructor
-  apply t_mem
-  unfold applySubstitutionTerm at v_t
-  cases t with
-  | constant c =>
-    simp at v_t
-    unfold termVariables at v_t
-    simp at v_t
-  | variableDL v' =>
-    unfold termVariables at v_t
-    simp at v_t
-    by_cases h: Option.isSome (s v') = true
-    simp [h] at v_t
-    simp [h] at v_t
-    rw [v_t]
-    unfold termVariables
-    simp
-    unfold substitution_domain
-    simp
-    cases h':s v' with
-    | some o =>
-      rw [h'] at h
-      simp at h
-    | none =>
-      simp
-
-  intro h
-  rw [← exists_and_right] at h
-  rcases h with ⟨t, h_t⟩
-  use t
-  simp [h_t]
-  rcases h_t with ⟨left, v_dom⟩
-  rcases left with ⟨t_terms, v_t⟩
-  unfold applySubstitutionTerm
-  unfold termVariables
-  cases t with
-  | constant c =>
-    simp
-    unfold termVariables at v_t
-    simp at v_t
-  | variableDL v' =>
-    simp
-    unfold termVariables at v_t
-    simp at v_t
-    unfold substitution_domain at v_dom
-    rw [Set.mem_setOf] at v_dom
-    rw [v_t] at v_dom
-    simp [v_dom]
-    apply v_t
-
-
-
-
-
-
-def groundingStep (s: substitution τ) (i: List (groundAtom τ)) (pgr: partialGroundRule τ i.toSet ) (hd: atom τ) (tl: List (atom τ)) (noVars: atomVariables (applySubstitutionAtom s hd) = ∅ ) (mem: atomWithoutVariablesToGroundAtom (applySubstitutionAtom s hd) noVars ∈ i): partialGroundRule τ i.toSet :=
-  have h: ∀ (ga : groundAtom τ), ga ∈ pgr.groundedBody ++ [atomWithoutVariablesToGroundAtom (applySubstitutionAtom s hd) noVars] → ga ∈ List.toSet i := by
-    intros ga
-    simp
-    intro h'
-    cases h' with
-    | inl ga_grounded =>
-      apply pgr.members ga ga_grounded
-    | inr ga_new =>
-      rw [ga_new]
-      rw [← List.toSet_mem]
-      apply mem
-  {head:= applySubstitutionAtom s pgr.head, groundedBody:= pgr.groundedBody ++ [atomWithoutVariablesToGroundAtom (applySubstitutionAtom s hd) noVars] , ungroundedBody := List.map (fun x => applySubstitutionAtom s x) tl, members := h}
-
-def groundingStepPreservesSafety (s: substitution τ) (i: List (groundAtom τ)) (pgr: partialGroundRule τ i.toSet ) (hd: atom τ) (tl: List (atom τ)) (noVars: atomVariables (applySubstitutionAtom s hd) = ∅ ) (mem: atomWithoutVariablesToGroundAtom (applySubstitutionAtom s hd) noVars ∈ i) (safe: pgr.isSafe) (h: pgr.ungroundedBody = hd::tl ): (groundingStep s i pgr hd tl noVars mem).isSafe := by
-  unfold partialGroundRule.isSafe
-  unfold groundingStep
-  simp
-  rw [applySubstitutionAtomRemovesDomainFromAtomVars,collectResultsToFinsetSemantics, Set.subset_def]
-  simp
-  intros v v_head v_dom
   unfold partialGroundRule.isSafe at safe
-  rw [collectResultsToFinsetSemantics, Set.subset_def] at safe
+  rw [body] at safe
+  unfold List.foldl_union at safe
   simp at safe
-  specialize safe v v_head
-  rcases safe with ⟨a, a_body, v_a⟩
-  rw [h] at a_body
-  simp at a_body
-  cases a_body with
-  | inl a_hd =>
-    rw [a_hd] at v_a
-    exfalso
-    rw [applySubstitutionAtomRemovesDomainFromAtomVars] at noVars
-    rw [Set.ext_iff] at noVars
-    specialize noVars v
-    simp at noVars
-    specialize noVars v_a
-    exact absurd noVars v_dom
-  | inr a_tl =>
-    use a
-    constructor
-    exact a_tl
-    rw [applySubstitutionAtomRemovesDomainFromAtomVars]
-    simp
-    constructor
-    apply v_a
-    apply v_dom
+  apply Finset.Subset.antisymm
+  apply safe
+  simp
 
-def atomVariablesEmpty.go (l: List (term τ)): Bool :=
-  match l with
-  | [] => true
-  | hd::tl =>
-    match hd with
-    | term.constant _ => atomVariablesEmpty.go tl
-    | term.variableDL _ => false
+def moveAtomWithoutVariables (pgr: partialGroundRule τ) (hd: atom τ) (tl: List (atom τ)) (noVars: atomVariables hd = ∅): partialGroundRule τ :=
+{
+  head := pgr.head,
+  groundedBody := pgr.groundedBody ++ [atomWithoutVariablesToGroundAtom hd noVars]
+  ungroundedBody := tl
+}
 
-def atomVariablesEmpty (a: atom τ): Bool := atomVariablesEmpty.go a.atom_terms
-
-lemma atomVariablesEmptyGoSemantics (l: List (term τ)): atomVariablesEmpty.go l = true ↔ collectResultsToFinset termVariables l = ∅  := by
-  induction l with
-  | nil =>
-    unfold atomVariablesEmpty.go
-    unfold collectResultsToFinset
-    simp
-  | cons hd tl ih =>
-    unfold atomVariablesEmpty.go
-    unfold collectResultsToFinset
-    cases hd with
-    | constant c =>
-      unfold termVariables
-      simp
-      unfold termVariables at ih
-      simp [ih]
-    | variableDL v =>
-      unfold termVariables
-      simp
-      rw [Set.ext_iff]
-      push_neg
-      simp
-
-
-lemma atomVariablesEmptySemantics (a: atom τ): atomVariablesEmpty a = true ↔ atomVariables a = ∅ :=
+lemma moveAtomWithoutVariablesPreservesSafety (pgr: partialGroundRule τ) (hd: atom τ) (tl: List (atom τ)) (body: pgr.ungroundedBody = hd::tl) (noVars: atomVariables hd = ∅) (safe: pgr.isSafe): (moveAtomWithoutVariables pgr hd tl noVars).isSafe :=
 by
-  unfold atomVariables
-  unfold atomVariablesEmpty
-  apply atomVariablesEmptyGoSemantics
-
-lemma groundingStepGroundAtomExtendMembers (i: List (groundAtom τ)) (pgr: partialGroundRule τ i.toSet ) (hd: groundAtom τ) (mem: hd ∈ i):  ∀ (ga : groundAtom τ), ga ∈ pgr.groundedBody ++ [hd] → ga ∈ List.toSet i:= by
-  intro ga
+  unfold partialGroundRule.isSafe at *
+  unfold moveAtomWithoutVariables
   simp
-  intro p
-  cases p with
-  | inl q =>
-    apply pgr.members
-    apply q
-  | inr q =>
-    rw [← List.toSet_mem,q]
-    apply mem
-
-lemma groundingStepGroundAtomExtendMembers_append (i: List (groundAtom τ)) (pgr: partialGroundRule τ i.toSet ) (hd: groundAtom τ) (mem: hd ∈ i):  ∀ (ga : groundAtom τ), ga ∈ (pgr.groundedBody ++ [hd]) → ga ∈ List.toSet i:= by
-  intro ga
-  simp
-  intro p
-  cases p with
-  | inl q =>
-    apply pgr.members
-    apply q
-  | inr q =>
-    rw [← List.toSet_mem,q]
-    apply mem
-
-def groundingStepGroundAtom (i: List (groundAtom τ)) (pgr: partialGroundRule τ i.toSet ) (hd: groundAtom τ) (tl: List (atom τ)) (mem: hd ∈ i): partialGroundRule τ i.toSet :=
-  {head:= pgr.head, groundedBody := pgr.groundedBody ++ [hd], ungroundedBody := tl, members := groundingStepGroundAtomExtendMembers i pgr hd mem}
-
-def groundingStepGroundAtomPreservesSafe (i: List (groundAtom τ)) (pgr: partialGroundRule τ i.toSet ) (hd: groundAtom τ) (tl: List (atom τ)) (mem: hd ∈ i) (safe: pgr.isSafe) (h: pgr.ungroundedBody = hd.toAtom::tl ): (groundingStepGroundAtom i pgr hd tl mem).isSafe :=
-by
-  unfold partialGroundRule.isSafe
-  unfold groundingStepGroundAtom
-  simp
-  unfold partialGroundRule.isSafe at safe
-  rw [h] at safe
-  unfold collectResultsToFinset at safe
-  rw [groundAtomsHaveNoVariables, Set.empty_union] at safe
+  rw [body] at safe
+  unfold List.foldl_union at safe
+  simp at safe
+  rw [noVars] at safe
+  unfold List.foldl_union
   apply safe
 
 
-def exploreGrounding (i: List (groundAtom τ)) (pgr: partialGroundRule τ i.toSet ) (safe: pgr.isSafe): Except String Unit :=
-  match h: pgr.ungroundedBody with
+def groundingStep (pgr: partialGroundRule τ) (hd: atom τ) (tl: List (atom τ)) (s: substitution τ) (noVars: atomVariables (applySubstitutionAtom s hd) = ∅ ): partialGroundRule τ :=
+{
+  head := applySubstitutionAtom s pgr.head,
+  groundedBody := pgr.groundedBody ++ [atomWithoutVariablesToGroundAtom (applySubstitutionAtom s hd) noVars],
+  ungroundedBody := List.map (applySubstitutionAtom s) tl
+}
+
+lemma groundingStepPreservesSafety (pgr: partialGroundRule τ) (hd: atom τ) (tl: List (atom τ)) (s: substitution τ) (noVars: atomVariables (applySubstitutionAtom s hd) = ∅ ) (safe: pgr.isSafe): (groundingStep pgr hd tl s noVars).isSafe :=
+by
+  unfold partialGroundRule.isSafe
+  unfold groundingStep
+  simp
+  rw [atomVariablesApplySubstitution]
+  admit
+
+
+
+def exploreGrounding (pgr: partialGroundRule τ) (i: List (groundAtom τ)) (safe: pgr.isSafe): Except String Unit :=
+  match h:pgr.ungroundedBody with
   | [] =>
-    have varHead: atomVariables pgr.head = ∅ := by
-      unfold partialGroundRule.isSafe at safe
-      rw [h] at safe
-      unfold collectResultsToFinset at safe
-      rw [Set.ext_iff]
-      simp
-      intro v
-      push_neg
-      rw [Set.subset_def] at safe
-      specialize safe v
-      apply safe
-    if (atomWithoutVariablesToGroundAtom pgr.head varHead) ∈ i
-    then Except.ok ()
-    else Except.error "Error"
+      let head' := atomWithoutVariablesToGroundAtom pgr.head (headOfSafePgrWithoutGroundedBodyHasNoVariables pgr safe h)
+
+      if head' ∈ i
+      then Except.ok ()
+      else Except.error ("Unfulfilled rule: " ++ ToString.toString pgr.toRule)
   | hd::tl =>
-    have noVars: ∀ (s: substitution τ), s ∈ getSubstitutions i hd → atomVariables (applySubstitutionAtom s hd) = ∅ := by
-      apply inGetSubstitutionsImplNoVars
-    if h': atomVariablesEmpty hd = true
+    if noVars:atomVariables hd = ∅
     then
-      have varsHd: atomVariables hd = ∅ := by
-        rw [atomVariablesEmptySemantics] at h'
-        apply h'
-      have uBody': pgr.ungroundedBody = (atomWithoutVariablesToGroundAtom hd varsHd).toAtom :: tl := by
-        rw [toAtomOfatomWithoutVariablesIsSelf]
-        apply h
-      if p: atomWithoutVariablesToGroundAtom hd varsHd ∈ i
-      then
-        exploreGrounding i (groundingStepGroundAtom i pgr (atomWithoutVariablesToGroundAtom hd varsHd) tl p) (groundingStepGroundAtomPreservesSafe i pgr (atomWithoutVariablesToGroundAtom hd varsHd) tl p safe uBody')
-      else
-        Except.ok ()
+      if atomWithoutVariablesToGroundAtom hd noVars ∈ i
+      then exploreGrounding (moveAtomWithoutVariables pgr hd tl noVars) i (moveAtomWithoutVariablesPreservesSafety pgr hd tl h noVars safe)
+      else Except.ok ()
     else
-      List.map_except_unit (getSubstitutions i hd).attach (fun ⟨s, _h⟩ => exploreGrounding i (groundingStep s i pgr hd tl (noVars s _h) (inGetSubstitutionsImplInInterpretation i hd s _h (noVars s _h))) (groundingStepPreservesSafety s i pgr hd tl (noVars s _h) (inGetSubstitutionsImplInInterpretation i hd s _h (noVars s _h)) safe h) )
+      List.map_except_unit (getSubstitutions i hd).attach (fun ⟨s, _h⟩ =>
+        let noVars':= inGetSubstitutionsImplNoVars i hd s _h
+        if atomWithoutVariablesToGroundAtom (applySubstitutionAtom s hd) noVars' ∈ i
+        then exploreGrounding (groundingStep pgr hd tl s noVars') i (groundingStepPreservesSafety pgr hd tl s noVars' safe)
+        else
+          Except.ok ()
+      )
 termination_by pgr.ungroundedBody.length
 decreasing_by
-  all_goals{
   simp_wf
-  simp [groundingStep, groundingStepGroundAtom, h]
-  }
-
-lemma applyGroundingTermEqtermWithoutVariablesToConstant (t: term τ) (noVars: termVariables t = ∅) (g: grounding τ): termWithoutVariablesToConstant t noVars = applyGroundingTerm' g t := by
-  cases t with
-  | constant c =>
-    unfold termWithoutVariablesToConstant
-    unfold applyGroundingTerm'
-    simp
-  | variableDL v =>
-    exfalso
-    unfold termVariables at noVars
-    simp at noVars
-
-lemma atomGroundingEqAtomWithoutVariablesToGroundAtom (a: atom τ) (noVars: atomVariables a = ∅) (g: grounding τ): atomWithoutVariablesToGroundAtom a noVars = atomGrounding g a := by
-  unfold atomWithoutVariablesToGroundAtom
-  unfold atomGrounding
-  rw [groundAtomEquality]
+  unfold moveAtomWithoutVariables
+  rw [h]
   simp
-  apply List.ext_get
-  rw [List.length_map, List.length_map, List.length_attach]
-  intros n h1 h2
-  rw [List.length_map, List.length_attach] at h1
-  rw [List.get_map, List.get_map]
+
+  simp_wf
+  unfold groundingStep
+  rw [h]
   simp
-  apply applyGroundingTermEqtermWithoutVariablesToConstant
 
+lemma applySubstitutionOnConstantIsSame (c: τ.constants) (s: substitution τ): applySubstitutionTerm s c = c := by
+  unfold applySubstitutionTerm
+  simp
 
-
-lemma atomGroundingIsSelfOnGroundAtom (ga: groundAtom τ) (g: grounding τ): atomGrounding g ga = ga := by
-  unfold atomGrounding
-  rw [groundAtomEquality]
+lemma applySubstitutionOnGroundAtomIsSame (ga: groundAtom τ) (s: substitution τ): applySubstitutionAtom s ga = ga := by
+  simp
   unfold groundAtom.toAtom
+  unfold applySubstitutionAtom
   simp
+
   apply List.ext_get
-  rw [List.length_map]
-  intros n h1 h2
-  rw [List.get_map]
   simp
-  unfold applyGroundingTerm'
+  intro n h1 h2
+  simp
+  rw [applySubstitutionOnConstantIsSame]
+
+
+lemma swapPgrApplySubstitution  (head hd: atom τ) (groundedBody: List (groundAtom τ)) (tl: List (atom τ))  (s: substitution τ) (noVars: atomVariables (applySubstitutionAtom s hd) = ∅): ({head:= applySubstitutionAtom s head, groundedBody:= groundedBody ++ [atomWithoutVariablesToGroundAtom (applySubstitutionAtom s hd) noVars], ungroundedBody:= List.map (applySubstitutionAtom s) tl}: partialGroundRule τ).toRule = applySubstitutionRule s (({head:=head, groundedBody:=groundedBody, ungroundedBody:=hd::tl}: partialGroundRule τ).toRule) := by
+  unfold partialGroundRule.toRule
+  unfold applySubstitutionRule
   simp
 
-lemma moveAtomWithoutVariablesInPartialGroundRule (i: List (groundAtom τ))(pgr: partialGroundRule τ i.toSet) (hd: atom τ) (tl: List (atom τ)) (h: pgr.ungroundedBody = hd::tl) (hdVars: atomVariables hd = ∅) (hd_i: atomWithoutVariablesToGroundAtom hd hdVars ∈ i): partialGroundRule.toRule pgr = partialGroundRule.toRule (i:= i.toSet) {head := pgr.head, groundedBody :=  pgr.groundedBody ++ [atomWithoutVariablesToGroundAtom hd hdVars], ungroundedBody := tl, members := groundingStepGroundAtomExtendMembers i pgr (atomWithoutVariablesToGroundAtom hd hdVars) hd_i} :=
-by
-  unfold partialGroundRule.toRule
-  simp
-  rw [h]
-  rw [toAtomOfatomWithoutVariablesIsSelf]
-
-lemma moveAtomWithoutVariablesInPartialGroundRule_singleElements (i: List (groundAtom τ))(head: atom τ) (groundedBody: List (groundAtom τ)) (hd: atom τ) (tl: List (atom τ)) (ungroundedBody: List (atom τ)) (members: ∀ (ga: groundAtom τ), ga ∈ groundedBody → ga ∈ List.toSet i) (h:ungroundedBody = hd::tl) (hdVars: atomVariables hd = ∅) (hd_i: atomWithoutVariablesToGroundAtom hd hdVars ∈ i): partialGroundRule.toRule {head:= head, groundedBody:= groundedBody, ungroundedBody:= ungroundedBody, members:= members} = partialGroundRule.toRule (i:= i.toSet) {head := head, groundedBody := groundedBody ++ [atomWithoutVariablesToGroundAtom hd hdVars], ungroundedBody := tl, members := groundingStepGroundAtomExtendMembers_append i {head:= head, groundedBody:= groundedBody, ungroundedBody:= ungroundedBody, members:= members} (atomWithoutVariablesToGroundAtom hd hdVars) hd_i} :=
-by
-  unfold partialGroundRule.toRule
-  simp
-  rw [h]
-  rw [toAtomOfatomWithoutVariablesIsSelf]
+  have h1:List.map groundAtom.toAtom groundedBody = List.map (applySubstitutionAtom s ∘ groundAtom.toAtom) groundedBody := by
+    apply List.ext_get
+    simp
+    intro n h1 h2
+    simp
+    rw [applySubstitutionOnGroundAtomIsSame]
+  rw [h1]
+  have h2: groundAtom.toAtom (atomWithoutVariablesToGroundAtom (applySubstitutionAtom s hd) noVars) = applySubstitutionAtom s hd := by
+    rw [← groundAtomToAtomOfAtomWithoutVariablesToGroundAtomIsSelf]
+  rw [h2]
 
 def combineSubstitutionGrounding (s: substitution τ) (g: grounding τ): grounding τ := fun x => if h: Option.isSome (s x) then Option.get (s x) h else g x
 
@@ -619,474 +365,237 @@ lemma combineSubstitutionGroundingEquivRule (r: rule τ) (s: substitution τ) (g
   intro n h1 h2
   simp [← List.map_map, List.get_map, combineSubstitutionGroundingEquivAtom]
 
-def decidableAtomVars.go (l: List (term τ)) (curr: List τ.vars): List τ.vars :=
-  match l with
-  | [] => curr
-  | hd::tl =>
-    match hd with
-    | term.constant _ => decidableAtomVars.go tl curr
-    | term.variableDL v => decidableAtomVars.go tl (curr.insert v)
-
-lemma decidableAtomVarsGoSemantics (l: List (term τ)) (curr: List τ.vars) (v: τ.vars): v ∈ decidableAtomVars.go l curr ↔ v ∈ curr ∨ v ∈ collectResultsToFinset termVariables l := by
-  induction l generalizing curr with
-  | nil =>
-    unfold collectResultsToFinset
-    unfold decidableAtomVars.go
-    simp
-  | cons hd tl ih =>
-    unfold decidableAtomVars.go
-    unfold collectResultsToFinset
-    rw [Set.mem_union, or_comm, or_assoc, or_comm (b:= v ∈ curr)]
-    cases hd with
-    | constant c =>
-      rw [ih]
-      unfold termVariables
-      simp
-    | variableDL w =>
-      specialize ih (List.insert w curr)
-      simp
-      rw [ih]
-      simp
-      have h: v ∈ termVariables (term.variableDL w) ↔ v = w := by
-        unfold termVariables
-        simp
-      rw [h]
-      rw [or_assoc]
-
-
-def decidableAtomVars (a: atom τ): List (τ.vars) := decidableAtomVars.go a.atom_terms []
-
-lemma inDecidableAtomVarsIffInAtomVariables (a: atom τ) (v: τ.vars): v ∈ atomVariables a ↔ v ∈ decidableAtomVars a := by
-  unfold decidableAtomVars
-  rw [decidableAtomVarsGoSemantics]
-  unfold atomVariables
-  simp
-
-def atomSubOfGrounding (a: atom τ) (g: grounding τ): substitution τ := fun x => if x ∈ decidableAtomVars a then some (g x) else none
-
-lemma atomSubOfGroundingEqOnTerm (a: atom τ) (g: grounding τ) (t: term τ) (mem: t ∈ a.atom_terms): applySubstitutionTerm (atomSubOfGrounding a g) t = term.constant (applyGroundingTerm' g t) := by
-  unfold atomSubOfGrounding
-  unfold applySubstitutionTerm
-  unfold applyGroundingTerm'
-  simp
-  cases t with
-  | constant c =>
-    simp
-  | variableDL v =>
-    simp
-    have v_atomVars: v ∈ decidableAtomVars a := by
-      rw [← inDecidableAtomVarsIffInAtomVariables]
-      unfold atomVariables
-      rw [collectResultsToFinsetSemantics, Set.mem_setOf]
-      use (term.variableDL v)
-      constructor
-      apply mem
-      unfold termVariables
-      simp
-
-    have h: Option.isSome (if v ∈ decidableAtomVars a then some (g v) else none) = true := by
-      rw [Option.isSome_iff_exists]
-      use (g v)
-      simp [v_atomVars]
-
-    simp [h]
-    simp [v_atomVars]
-
-
-lemma atomSubOfGroundingEqOnAtom (a: atom τ) (g: grounding τ): applySubstitutionAtom (atomSubOfGrounding a g) a = atomGrounding g a := by
-  unfold applySubstitutionAtom
-  unfold atomGrounding
-  unfold groundAtom.toAtom
-  simp
-  apply List.ext_get
-  rw [List.length_map, List.length_map]
-  intro n h1 h2
-  rw [List.get_map, List.get_map]
-  apply atomSubOfGroundingEqOnTerm
-  simp
-  apply List.get_mem
-
-lemma atomSubOfGroundingGroundingEqGroundingOnTerm (a : atom τ)  (g: grounding τ) (t: term τ): applyGroundingTerm' g (applySubstitutionTerm (atomSubOfGrounding a g) t) = applyGroundingTerm' g t := by
-  unfold applyGroundingTerm'
-  unfold applySubstitutionTerm
-  unfold atomSubOfGrounding
-  cases t with
-  | constant c =>
-    simp
-  | variableDL v =>
-    simp
-    by_cases h: Option.isSome (if v ∈ decidableAtomVars a then some (g v) else none) = true
-    simp [h]
-    by_cases p: v ∈ decidableAtomVars a
-    simp [p]
-    simp [p] at h
-    simp [h]
-
-
-lemma atomSubOfGroundingGroundingEqGroundingOnAtom (a a': atom τ)  (g: grounding τ) : atomGrounding g (applySubstitutionAtom (atomSubOfGrounding a g) a') = atomGrounding g a' := by
-  unfold atomGrounding
-  unfold applySubstitutionAtom
-  simp
-  apply List.ext_get
-  rw [List.length_map, List.length_map]
-
-  intro n h1 h2
-  simp [← List.map_map]
-  simp [atomSubOfGroundingGroundingEqGroundingOnTerm]
-
-
-lemma atomSubOfGroundingGroundingEqGroundingOnRule (a: atom τ) (g: grounding τ) (r: rule τ): ruleGrounding (applySubstitutionRule (atomSubOfGrounding a g) r) g = ruleGrounding r g := by
-  unfold ruleGrounding
-  unfold applySubstitutionRule
-  simp
+lemma replaceGroundingWithSubstitutionAndGrounding (a: atom τ) (r: rule τ) (mem: a ∈ r.body ): (∀ (g: grounding τ),   ruleTrue (ruleGrounding r g) i) ↔ ∀ (s: substitution τ), (∃ (ga: groundAtom τ), ga ∈ i ∧ applySubstitutionAtom s a = ga ∧ ∀ (s': substitution τ), applySubstitutionAtom s' a = ga → s ⊆ s') →  ∀ (g': grounding τ),ruleTrue (ruleGrounding (applySubstitutionRule s r) g') i := by
   constructor
-  apply atomSubOfGroundingGroundingEqGroundingOnAtom
-
-  apply List.ext_get
-  rw [List.length_map, List.length_map]
-  intros n h1 h2
-  rw [List.get_map, List.get_map]
-  simp [atomSubOfGroundingGroundingEqGroundingOnAtom]
-
-lemma equalOfListMapEqual {A B: Type} (l:List A) (f g: A → B) (h: List.map f l = List.map g l) (a: A) (mem: a ∈ l): f a = g a := by
-  induction l with
-  | nil =>
-    simp at mem
-  | cons hd tl ih =>
-    simp at mem
-    simp at h
-    cases mem with
-    | inl p =>
-      rw [← p] at h
-      simp [h]
-    | inr p =>
-      apply ih
-      simp [h]
-      apply p
-
-lemma variableMemberOfcollecResultsIffMemberList (l: List (term τ)) (v: τ.vars): term.variableDL v ∈ l ↔ v ∈ collectResultsToFinset termVariables l := by
-  induction l with
-  | nil =>
-    unfold collectResultsToFinset
-    simp
-  | cons hd tl ih =>
-    unfold collectResultsToFinset
-    simp
-    rw [← ih]
-    unfold termVariables
-    simp
-    cases hd with
-    | constant c =>
-      simp
-    | variableDL w =>
-      simp
-
-
-lemma atomSubOfGroundingIsMinimalForAtom (a: atom τ) (g: grounding τ):
-(∀ (s' : substitution τ), applySubstitutionAtom s' a = groundAtom.toAtom (atomGrounding g a) → atomSubOfGrounding a g ⊆ s') := by
-  intro s' s'_a
-  unfold_projs
-  unfold substitution_subs
-  intro v
-  intro h'
-  unfold substitution_domain at h'
-  simp at h'
-  unfold atomSubOfGrounding
-  cases h:(atomSubOfGrounding a g v) with
-  | some c =>
-    unfold atomSubOfGrounding at h
-    have p: v ∈ decidableAtomVars a := by
-      by_contra q
-      simp [q] at h
-    simp [p] at h
-    rw [← inDecidableAtomVarsIffInAtomVariables] at p
-    unfold applySubstitutionAtom at s'_a
-    unfold atomGrounding at s'_a
-    unfold groundAtom.toAtom at s'_a
-    simp at s'_a
-    have s'_v: applySubstitutionTerm s' (term.variableDL v) = (term.constant ∘ applyGroundingTerm' g) (term.variableDL v) := by
-      apply equalOfListMapEqual (h:= s'_a)
-      rw [variableMemberOfcollecResultsIffMemberList]
-      unfold atomVariables at p
-      apply p
-    unfold applySubstitutionTerm at s'_v
-    unfold applyGroundingTerm' at s'_v
-    simp at s'_v
-    cases h': (s' v) with
-    | some c' =>
-      simp [h'] at s'_v
-      rw [h] at s'_v
-      simp
-      rw [inDecidableAtomVarsIffInAtomVariables] at p
-      simp [p]
-      rw [h]
-      apply Eq.symm
-      apply s'_v
-    | none =>
-      simp [h'] at *
-  | none =>
-    rw [h] at h'
-    simp at h'
-
-lemma replaceGroundingWithSubstitutionAndGrounding (a: atom τ) (r: rule τ) (mem: a ∈ r.body ): (∀ (g: grounding τ), atomGrounding g a ∈ i →  ruleTrue (ruleGrounding r g) i) ↔ ∀  (s: substitution τ), (∃ (ga: groundAtom τ), ga ∈ i ∧ applySubstitutionAtom s a = ga ∧ ∀ (s': substitution τ), applySubstitutionAtom s' a = ga → s ⊆ s') →  ∀ (g': grounding τ),ruleTrue (ruleGrounding (applySubstitutionRule s r) g') i := by
-  constructor
-  intros h s _ g
+  intro h s s_prop g'
   rw [combineSubstitutionGroundingEquivRule]
-  by_cases p: atomGrounding (combineSubstitutionGrounding s g) a ∈ i
   apply h
-  apply p
+
+  intro h g
+  by_cases g_a_i: atomGrounding g a ∈ i
+  admit
+
   unfold ruleTrue
-  unfold groundRuleBodySet
-  unfold ruleGrounding
-  rw [Set.subset_def]
-  intro q
-  specialize q (atomGrounding (combineSubstitutionGrounding s g) a)
-  simp at q
-  exfalso
-  specialize q a mem
-  simp at q
-  exact absurd q p
-
-  intros h g ground_g_a
-  specialize h (atomSubOfGrounding a g)
-  simp at h
-  specialize h (atomGrounding g a) ground_g_a  (atomSubOfGroundingEqOnAtom a g)
-  specialize h (atomSubOfGroundingIsMinimalForAtom a g) g
-  rw [atomSubOfGroundingGroundingEqGroundingOnRule] at h
-  apply h
-
-lemma swapApplySubstitutionPgrToRule (i: List (groundAtom τ)) (s: substitution τ) (pgr: partialGroundRule τ i.toSet) (hd: atom τ) (tl: List (atom τ)) (varsHd: atomVariables (applySubstitutionAtom s hd) = ∅) (mem: (atomWithoutVariablesToGroundAtom (applySubstitutionAtom s hd) varsHd) ∈ i) (h: pgr.ungroundedBody = hd::tl): applySubstitutionRule s (pgr.toRule) = partialGroundRule.toRule {head:= applySubstitutionAtom s pgr.head, groundedBody:= pgr.groundedBody ++ [atomWithoutVariablesToGroundAtom (applySubstitutionAtom s hd) varsHd], ungroundedBody:= List.map (applySubstitutionAtom s) tl, members:= groundingStepGroundAtomExtendMembers i pgr (atomWithoutVariablesToGroundAtom (applySubstitutionAtom s hd) varsHd) mem} :=
-by
-  unfold partialGroundRule.toRule
-  unfold applySubstitutionRule
-  rw [h]
-  simp
-  rw [toAtomOfatomWithoutVariablesIsSelf]
-  have groundedBodyEq:  List.map (applySubstitutionAtom s ∘ groundAtom.toAtom) pgr.groundedBody = List.map groundAtom.toAtom pgr.groundedBody := by
-    apply List.ext_get
-    rw [List.length_map, List.length_map]
-    intros n h1 h2
-    rw [List.get_map, List.get_map]
-    simp
-    have p: ∀ (ga:groundAtom τ), applySubstitutionAtom s (groundAtom.toAtom ga) = groundAtom.toAtom ga := by
-      intro ga
-      unfold groundAtom.toAtom
-      unfold applySubstitutionAtom
-      simp
-      apply List.ext_get
-      rw [List.length_map, List.length_map]
-      intros n' h1' h2'
-      rw [List.get_map, List.get_map]
-      simp
-      have q: ∀ (c: τ.constants), applySubstitutionTerm s (term.constant c) =term.constant c := by
-        intro c
-        unfold applySubstitutionTerm
-        simp
-      rw [q]
-    rw [p]
-  rw [groundedBodyEq]
+  intro bodySet
+  rw [Set.subset_def] at bodySet
+  simp at bodySet
+  specialize bodySet (atomGrounding g a)
+  rw [← groundRuleBodySet_iff_groundRuleBody] at bodySet
+  unfold ruleGrounding at bodySet
+  simp at bodySet
+  specialize bodySet a mem
+  simp at bodySet
+  contradiction
 
 
-theorem exploreGroundingSemantics (i: List (groundAtom τ)) (pgr: partialGroundRule τ i.toSet ) (safe: pgr.isSafe): exploreGrounding i pgr safe = Except.ok () ↔ pgr.isTrue := by
-  unfold partialGroundRule.isTrue
+
+theorem exploreGroundingSemantics (i: List (groundAtom τ)) (pgr: partialGroundRule τ) (safe: pgr.isSafe) (active: pgr.isActive i.toSet): exploreGrounding pgr i safe = Except.ok () ↔ pgr.isTrue i.toSet := by
   cases pgr with
-  | mk head groundedBody ungroundedBody members =>
-    induction' length: ungroundedBody.length with n ih generalizing head groundedBody ungroundedBody members
+  | mk head groundedBody ungroundedBody =>
+    induction' length: ungroundedBody.length with n ih generalizing head groundedBody ungroundedBody
 
+    rw [List.length_eq_zero] at length
+    simp_rw [length]
     unfold exploreGrounding
     simp
-    cases ungroundedBody with
-    | cons hd tl =>
-      simp at length
-    | nil =>
-      simp
-      unfold ruleTrue
-      unfold partialGroundRule.toRule
-      simp
-      unfold partialGroundRule.isSafe at safe
-      unfold collectResultsToFinset at safe
-      rw [Set.subset_empty_iff] at safe
-      simp at safe
-      unfold ruleGrounding
-      simp [imp_false, ← atomGroundingEqAtomWithoutVariablesToGroundAtom head safe, ← List.toSet_mem]
-      constructor
-      intros h' _ _
-      simp [h']
-      intro h'
-      apply h'
-      unfold groundRuleBodySet
-      simp
-      rw [Set.subset_def]
-      intro ga body
-      apply members
-      have groundingBody: ∀ (g: grounding τ), List.map (atomGrounding g ∘ groundAtom.toAtom ) groundedBody = groundedBody := by
-        intro g
-        apply List.ext_get
-        rw [List.length_map]
-        intros n h1 h2
-        rw [List.get_map]
+    unfold partialGroundRule.isTrue
+    simp_rw [groundingOnPartialGroundRule]
+    unfold ruleTrue
+    simp
+    simp_rw [← List.toSet_mem]
+    have bodyEmpty: ({head:=head, groundedBody := groundedBody, ungroundedBody := ungroundedBody}:partialGroundRule τ).ungroundedBody = [] :=
+      by
         simp
-        rw [atomGroundingIsSelfOnGroundAtom]
-      simp [groundingBody, atomGroundingIsSelfOnGroundAtom] at body
-      apply body
-      use (substitutionToGrounding emptySubstitution) -- we have to use some substitution
+        exact length
+    have h': head = atomWithoutVariablesToGroundAtom head (headOfSafePgrWithoutGroundedBodyHasNoVariables {head:=head, groundedBody := groundedBody, ungroundedBody := ungroundedBody} safe bodyEmpty) := by
+      simp
+      rw [← groundAtomToAtomOfAtomWithoutVariablesToGroundAtomIsSelf]
+    unfold groundRuleBodySet
+    simp
+    constructor
+    intro h g _
+    rw [h']
+    simp
+    rw [atomGroundingOnGroundAtomReturnsSame]
+    apply h
+    intro h
+    specialize h (substitutionToGrounding emptySubstitution)
+    have subs: {a | a ∈ groundedBody} ⊆ List.toSet i := by
+      rw [Set.subset_def]
+      intro a
+      simp
+      intro a_mem
+      unfold partialGroundRule.isActive at active
+      apply active
+      simp
+      exact a_mem
+    specialize h subs
+    rw [h'] at h
+    simp at h
+    rw [atomGroundingOnGroundAtomReturnsSame] at h
+    exact h
 
     unfold exploreGrounding
-    simp
     cases ungroundedBody with
-    | nil =>
-      exfalso
-      simp at length
+    | nil => simp at length
     | cons hd tl =>
       simp
       simp at length
-      constructor
-      intros h' g
-      by_cases varsHd: atomVariablesEmpty hd = true
-      simp [varsHd] at h'
-      rw [atomVariablesEmptySemantics] at varsHd
-      by_cases hd_i: atomWithoutVariablesToGroundAtom hd varsHd ∈ i
-      specialize h' hd_i
-      unfold groundingStepGroundAtom  at h'
-      rw [ih] at h'
-      simp at h'
-      specialize h' g
-      rw [moveAtomWithoutVariablesInPartialGroundRule (hd:= hd)  (tl:=tl) (hdVars:= varsHd) (hd_i:= hd_i)]
+      split
+      rename_i noVars
+
+      by_cases hd_i: (atomWithoutVariablesToGroundAtom hd noVars) ∈ i
+      simp [hd_i]
+      unfold moveAtomWithoutVariables
       simp
-      apply h'
-      simp
-      apply length
-      unfold ruleGrounding
-      unfold ruleTrue
-      unfold partialGroundRule.toRule
-      simp
-      unfold groundRuleBodySet
-      simp
-
-      rw [Set.subset_def]
-      intro body
-      specialize body (atomWithoutVariablesToGroundAtom hd varsHd)
-      simp [Finset.mem_insert] at body
-      have n_hd_i: atomWithoutVariablesToGroundAtom hd varsHd ∈ i := by
-        rw [List.toSet_mem]
-        apply body
-        left
-        rw [atomGroundingEqAtomWithoutVariablesToGroundAtom]
-      exfalso
-      exact absurd n_hd_i hd_i
-
-      simp [varsHd] at h'
-      rw [List.map_except_unitIsUnitIffAll] at h'
-      by_cases g_hd: atomGrounding g hd ∈ i
-      revert g
-      simp [List.toSet_mem]
-      rw [replaceGroundingWithSubstitutionAndGrounding (a:=hd)]
-      intros s s_prop
-      rw [←  inGetSubstitutionsIffMinimalSolutionAndInInterpretation] at s_prop
-      specialize h' (Subtype.mk s s_prop)
-      unfold groundingStep at h'
-      simp at h'
-      rw [inGetSubstitutionsIffMinimalSolutionAndInInterpretation] at s_prop
-      simp at s_prop
-      rcases s_prop with ⟨ga, ga_i, apply_s_ga, _⟩
-      have varsHdS: atomVariables (applySubstitutionAtom s hd) = ∅ := by
-        rw [apply_s_ga]
-        apply groundAtomsHaveNoVariables
-
-      rw [swapApplySubstitutionPgrToRule (hd:=hd) (tl:= tl) (varsHd:= varsHdS)]
-      simp
-      rw [← ih]
-      rw [← h']
-
-      simp [apply_s_ga, atomWithoutVariablesToGroundAtomOfGroundAtom]
-      rw [List.toSet_mem]
-      apply ga_i
-
-      rw [List.length_map]
-      apply length
-
-      simp
-
-      unfold partialGroundRule.toRule
-      simp
-
-      unfold partialGroundRule.toRule
-      unfold ruleGrounding
-      unfold ruleTrue
-      unfold groundRuleBodySet
-      rw [Set.subset_def]
-      simp
-      intro body
-      rw [← List.toSet_mem] at body
-      exfalso
-      exact absurd body g_hd
-
-      -- back direction
-      intro h'
-      by_cases varsHd: atomVariablesEmpty hd = true
-      simp [varsHd]
-      intro hd_i
       rw [ih]
-      unfold groundingStepGroundAtom
+      apply partialGroundRule.isTrue_of_equal_toRule
+      unfold partialGroundRule.toRule
       simp
-      rw [atomVariablesEmptySemantics] at varsHd
-      rw [← moveAtomWithoutVariablesInPartialGroundRule_singleElements (hd:= hd) (tl:=tl) (ungroundedBody:= hd::tl) (hdVars:= varsHd) (hd_i:= hd_i)]
-      apply h'
-      rfl
-
-      unfold groundingStepGroundAtom
+      rw [← groundAtomToAtomOfAtomWithoutVariablesToGroundAtomIsSelf]
+      unfold partialGroundRule.isActive
+      intro ga
       simp
-      apply length
+      intro h
+      cases h with
+      | inl ga_body =>
+        apply active
+        simp
+        exact ga_body
+      | inr ga_hd =>
+        rw [ga_hd]
+        rw [← List.toSet_mem]
+        exact hd_i
+      exact length
 
-      simp [varsHd]
+      simp[hd_i]
+      unfold partialGroundRule.isTrue
+      intro g
+      unfold ruleTrue
+      rw [groundingOnPartialGroundRule]
+      simp
+      intro body_subs
+      rw [Set.subset_def] at body_subs
+      simp at body_subs
+      specialize body_subs (atomWithoutVariablesToGroundAtom hd noVars)
+      rw [← groundRuleBodySet_iff_groundRuleBody] at body_subs
+      simp at body_subs
+      have n_hd_i: atomWithoutVariablesToGroundAtom hd noVars ∈  i:= by
+        rw [List.toSet_mem]
+        apply body_subs
+        right
+        left
+
+        admit
+      contradiction
+
       rw [List.map_except_unitIsUnitIffAll]
-      intro s _
-      rcases s with ⟨s,s_prop⟩
+      simp
       unfold groundingStep
       simp
-      rw [ih]
-      intro g
-      rw [← swapApplySubstitutionPgrToRule (pgr := {head:= head, groundedBody:=groundedBody, ungroundedBody:= hd::tl, members := members}) (hd:= hd) (tl:=tl) ]
-      rw [combineSubstitutionGroundingEquivRule]
-      apply h'
-
-      rw [inGetSubstitutionsIffMinimalSolutionAndInInterpretation] at s_prop
-      simp at s_prop
-      rcases s_prop with ⟨ga, ga_i, apply_s, _⟩
-      simp [apply_s]
-      rw [atomWithoutVariablesToGroundAtomOfGroundAtom]
-      rw [List.toSet_mem]
-      apply ga_i
-
+      constructor
+      intro h
+      unfold partialGroundRule.isTrue
+      rw [replaceGroundingWithSubstitutionAndGrounding (a:=hd)]
+      simp
+      intro s ga ga_i s_hd_ga s_min
+      specialize h s
+      have s_getSubs: s ∈ getSubstitutions i hd := by
+        rw [inGetSubstitutionsIffMinimalSolutionAndInInterpretation]
+        simp
+        use ga
+      specialize h s_getSubs
+      rw [ih] at h
+      unfold partialGroundRule.isTrue at h
+      rw [swapPgrApplySubstitution] at h
+      apply h
+      apply inGetSubstitutionsImplInInterpretation
+      exact s_getSubs
+      unfold partialGroundRule.isActive
+      simp
+      intro ga ga_mem
+      cases ga_mem with
+      | inl ga_body =>
+        unfold partialGroundRule.isActive at active
+        apply active
+        simp
+        exact ga_body
+      | inr ga_hd =>
+        rw [ga_hd]
+        rw [← List.toSet_mem]
+        apply inGetSubstitutionsImplInInterpretation
+        exact s_getSubs
+      simp
+      exact length
+      unfold partialGroundRule.toRule
       simp
 
-      rw [List.length_map]
-      apply length
+      intro h s s_mem s_hd_i
+      rw [ih]
+      unfold partialGroundRule.isTrue
+      intro g
+      rw [swapPgrApplySubstitution, combineSubstitutionGroundingEquivRule]
+      unfold partialGroundRule.isTrue at h
+      apply h
 
-lemma safePreservedBetweenRuleAndPartialGroundRule (r: rule τ) (i: interpretation τ): r.isSafe ↔ (partialGroundRuleFromRule r i).isSafe := by
+      unfold partialGroundRule.isActive
+      simp
+      intro ga ga_mem
+      cases ga_mem with
+      | inl ga_body =>
+        apply active
+        simp
+        exact ga_body
+      | inr ga_hd =>
+        rw [ga_hd]
+        rw [← List.toSet_mem]
+        exact s_hd_i
+      simp
+      exact length
+
+
+
+lemma safePreservedBetweenRuleAndPartialGroundRule (r: rule τ) : r.isSafe ↔ (partialGroundRule.fromRule r).isSafe := by
   unfold partialGroundRule.isSafe
   unfold rule.isSafe
-  unfold partialGroundRuleFromRule
+  unfold partialGroundRule.fromRule
   simp
 
 def modelChecker (i: List (groundAtom τ)) (P: List (rule τ)) (safe: ∀ (r: rule τ), r ∈ P → r.isSafe): Except String Unit :=
-  have safe': ∀ (r: rule τ), r ∈ P → (partialGroundRuleFromRule r i.toSet ).isSafe := by
+  have safe': ∀ (r: rule τ), r ∈ P → (partialGroundRule.fromRule r).isSafe := by
     intros r rP
     rw [← safePreservedBetweenRuleAndPartialGroundRule]
     apply safe r rP
-  List.map_except_unit P.attach (fun ⟨x, _h⟩ => exploreGrounding i (partialGroundRuleFromRule x i.toSet ) (safe' x _h) )
+  List.map_except_unit P.attach (fun ⟨x, _h⟩ => exploreGrounding (partialGroundRule.fromRule x ) i (safe' x _h) )
 
 theorem modelCheckerUnitIffAllRulesTrue (i: List (groundAtom τ)) (P: List (rule τ)) (safe: ∀ (r: rule τ), r ∈ P → r.isSafe): modelChecker i P safe = Except.ok () ↔ (∀ (r: groundRule τ), r ∈ groundProgram P.toFinset → ruleTrue r i.toSet) :=
 by
   unfold modelChecker
   rw [List.map_except_unitIsUnitIffAll]
-  simp [exploreGroundingSemantics, partialGroundRule.isTrue, groundProgram, ← partialGroundRuleToRuleInverseToFromRule]
+  simp
   constructor
-  intros h gr r rP g gr_r
-  rw [gr_r]
-  apply h r rP
+  intro h gr grP
+  unfold groundProgram at grP
+  simp at grP
+  rcases grP with ⟨r, rP, g, r_g⟩
+  specialize h r rP
+  rw [exploreGroundingSemantics] at h
+  unfold partialGroundRule.isTrue at h
+  specialize h g
+  rw [← partialGroundRuleToRuleInverseToFromRule, ← r_g] at h
+  exact h
+  apply partialGroundRule.fromRuleIsActive
 
-  intros h r rP g
+  intro h r rP
+  rw [exploreGroundingSemantics]
+  unfold partialGroundRule.isTrue
+  intro g
+  rw [← partialGroundRuleToRuleInverseToFromRule]
   specialize h (ruleGrounding r g)
-  apply h r rP g
-  rfl
+  apply h
+  unfold groundProgram
+  simp
+  use r
+  simp[*]
+  use g
+  apply partialGroundRule.fromRuleIsActive
